@prefix dbpedia: <http://dbpedia.org/ontology/> .
@prefix dcterms: <http://purl.org/dc/terms/> .
@prefix foaf: <http://xmlns.com/foaf/0.1/> .
@prefix nobel: <http://data.nobelprize.org/terms/> .
@prefix nobel-ext: <http://data.nobelprize.org/terms-ext/> .
@prefix owl: <http://www.w3.org/2002/07/owl#> .
@prefix rdf: <http://www.w3.org/1999/02/22-rdf-syntax-ns#> .
@prefix rdfs: <http://www.w3.org/2000/01/rdf-schema#> .
@prefix sh: <http://www.w3.org/ns/shacl#> .
@prefix skos: <http://www.w3.org/2004/02/skos/core#> .
@prefix xsd: <http://www.w3.org/2001/XMLSchema#> .

nobel-ext:AwardFileShape a sh:NodeShape;
  sh:property [ a sh:PropertyShape;
      sh:class nobel:FileType;
      sh:maxCount 1;
      sh:minCount 1;
      sh:path nobel:fileType
    ], [ a sh:PropertyShape;
      sh:datatype xsd:integer;
      sh:maxCount 1;
      sh:minCount 1;
      sh:path nobel:year
    ];
  sh:targetClass nobel:AwardFile .

nobel-ext:DBpediaLaureateAwardShape a sh:NodeShape;
  sh:property nobel-ext:FieldPropertyShape;
  sh:targetClass dbpedia:Award .

nobel-ext:FieldPropertyShape a sh:PropertyShape;
  sh:datatype xsd:string;
  sh:path nobel:field .

nobel-ext:LaureateAwardShape a sh:NodeShape;
  sh:property nobel-ext:LaureateAwardShape-awardFile, nobel-ext:LaureateAwardShape-category,
    nobel-ext:LaureateAwardShape-contribution, nobel-ext:LaureateAwardShape-isPartOf,
    nobel-ext:LaureateAwardShape-laureate, nobel-ext:LaureateAwardShape-motivation, nobel-ext:LaureateAwardShape-share,
    nobel-ext:LaureateAwardShape-university, nobel-ext:LaureateAwardShape-year;
  sh:targetClass nobel:LaureateAward .

nobel-ext:LaureateAwardShape-awardFile a sh:PropertyShape;
  sh:class nobel:AwardFile;
  sh:minCount 1;
  sh:path nobel:prizeFile .

nobel-ext:LaureateAwardShape-category a sh:PropertyShape;
  sh:class nobel:Category;
  sh:maxCount 1;
  sh:minCount 1;
  sh:path nobel:category .

nobel-ext:LaureateAwardShape-contribution a sh:PropertyShape;
  sh:datatype xsd:string;
  sh:maxCount 1;
  sh:path nobel:contribution .

nobel-ext:LaureateAwardShape-isPartOf a sh:PropertyShape;
  sh:class nobel:NobelPrize;
  sh:maxCount 1;
  sh:minCount 1;
  sh:path dcterms:isPartOf .

nobel-ext:LaureateAwardShape-laureate a sh:PropertyShape;
  sh:class nobel:Laureate;
  sh:maxCount 1;
  sh:minCount 1;
  sh:path nobel:laureate .

nobel-ext:LaureateAwardShape-motivation a sh:PropertyShape;
  sh:datatype xsd:string;
  sh:path nobel:motivation;
  sh:uniqueLang true .

nobel-ext:LaureateAwardShape-share a sh:PropertyShape;
  sh:datatype xsd:integer;
  sh:maxCount 1;
  sh:minCount 1;
  sh:path nobel:share .

nobel-ext:LaureateAwardShape-university a sh:PropertyShape;
  sh:class dbpedia:University;
  sh:path nobel:university .

nobel-ext:LaureateAwardShape-year a sh:PropertyShape;
  sh:datatype xsd:integer;
  sh:maxCount 1;
  sh:minCount 1;
  sh:path nobel:year .

nobel-ext:LaureateShape a sh:NodeShape;
  sh:property nobel-ext:LaureateShape-name, nobel-ext:LaureateShape-nobelPrize;
  sh:targetClass nobel:Laureate .

nobel-ext:LaureateShape-name a sh:PropertyShape;
  sh:datatype xsd:string;
  sh:maxCount 1;
  sh:minCount 1;
  sh:path foaf:name .

nobel-ext:LaureateShape-nobelPrize a sh:PropertyShape;
  sh:class nobel:NobelPrize;
  sh:message "every laureate should have at least one prize";
  sh:minCount 1;
  sh:path nobel:nobelPrize .

nobel-ext:NobelPrizeShape a sh:NodeShape;
  sh:property nobel-ext:NobelPrizeShape-category, nobel-ext:NobelPrizeShape-prizefile;
  sh:targetClass nobel:NobelPrize .

nobel-ext:NobelPrizeShape-category a sh:PropertyShape;
  sh:class nobel:Category;
  sh:maxCount 1;
  sh:message "every prize should have exactly one category";
  sh:minCount 1;
  sh:path nobel:category .

nobel-ext:NobelPrizeShape-prizefile a sh:PropertyShape;
  sh:class nobel:PrizeFile;
  sh:minCount 1;
  sh:path nobel:prizeFile .

nobel-ext:PersonShape a sh:NodeShape;
  sh:property nobel-ext:PersonShape-affiliation, nobel-ext:PersonShape-birthPlace, nobel-ext:PersonShape-dateOfBirth,
    nobel-ext:PersonShape-dateOfDeath, nobel-ext:PersonShape-deathPlace, nobel-ext:PersonShape-familyName,
    nobel-ext:PersonShape-givenName;
  sh:targetClass foaf:Person .

nobel-ext:PersonShape-affiliation a sh:PropertyShape;
  sh:class dbpedia:University;
  sh:path dbpedia:affiliation .

nobel-ext:PersonShape-birthPlace a sh:PropertyShape;
  sh:and ([
        sh:class dbpedia:Country;
        sh:maxCount 1;
        sh:minCount 1
      ] [
        sh:class dbpedia:City;
        sh:maxCount 1;
        sh:minCount 1
      ]);
  sh:path dbpedia:birthPlace .

nobel-ext:PersonShape-dateOfBirth a sh:PropertyShape;
  sh:datatype xsd:date;
  sh:maxCount 1;
  sh:minCount 1;
  sh:path dbpedia:dateOfBirth .

nobel-ext:PersonShape-dateOfDeath a sh:PropertyShape;
  sh:datatype xsd:date;
  sh:maxCount 1;
  sh:path dbpedia:dateOfDeath .

nobel-ext:PersonShape-deathPlace a sh:PropertyShape;
  sh:and ([
        sh:class dbpedia:Country;
        sh:maxCount 1
      ] [
        sh:class dbpedia:City;
        sh:maxCount 1
      ]);
  sh:path dbpedia:deathPlace .

nobel-ext:PersonShape-familyName a sh:PropertyShape;
  sh:datatype xsd:string;
  sh:maxCount 1;
  sh:minCount 1;
  sh:path foaf:familyName .

nobel-ext:PersonShape-givenName a sh:PropertyShape;
  sh:datatype xsd:string;
  sh:maxCount 1;
  sh:minCount 1;
  sh:path foaf:givenName .

nobel-ext:PrizeFileShape a sh:NodeShape;
  sh:property [ a sh:PropertyShape;
      sh:datatype xsd:integer;
      sh:maxCount 1;
      sh:minCount 1;
      sh:path nobel:year
    ], [ a sh:PropertyShape;
      sh:class nobel:FileType;
      sh:maxCount 1;
      sh:minCount 1;
      sh:path nobel:fileType
    ];
  sh:targetClass nobel:PrizeFile .

nobel-ext:Test a owl:Class;
  rdfs:isDefinedBy <http://data.nobelprize.org/terms/>;
  rdfs:label "Testing Testing" .

<http://data.nobelprize.org/terms/> a owl:Ontology;
  dcterms:contributor "Jeen Broekstra <jb@metaphacts.com>", "Johannes Trame <jt@metaphacts.com>";
  dcterms:created "2013-02-12T23:00:00.000Z"^^xsd:dateTime;
  dcterms:creator "nobelprize.org";
  dcterms:description """This ontology specifies the classes and properties to describe the nobel prize dataset.
  The nobel prize linked data dataset contains the authoritative information about Nobel prizes and Nobel Laureates since 1901.
  Please refer to https://www.nobelprize.org/about/linked-data-documentation/ for details.
  """@en;
  dcterms:title "Linked Nobelprize Ontology"@en;
  <http://www.linkedmodel.org/1.2/schema/vaem#namespace> <http://data.nobelprize.org/terms-ext/>;
  rdfs:comment """
  The original ontology was retrieved from http://data.nobelprize.org/terms/ in RDF/XML (Nov 2020).
  The ontology was converted into turtle and the following changes have been made by metaphacts:
  <li>
   <ul>Fix typo: nobel:Litterature -> nobel:Literature (correct in data, c.f. http://data.nobelprize.org/page/category/Literature)</ul>
   <ul>Added dedicated imports (FOAF, SKOS), define http://data.nobelprize.org/terms-ext/ as dedicated element namespace</ul>
   <ul>Added SHACL shapes and minor extensions (using http://data.nobelprize.org/terms-ext/ as element namespace)</ul>
  </li>
  The license is CC-BY 4.0 according to https://data.nobelprize.org/specification/ (January 2021).
  """@en;
  rdfs:seeAlso <http://www.nobelprize.org/>;
  owl:imports <http://www.w3.org/2004/02/skos/core>, <http://xmlns.com/foaf/0.1/>;
  owl:versionInfo "version 0.1" .

nobel:AwardFile a owl:Class;
  rdfs:comment "Some form of media related to the award given to a specific Laureate.";
  rdfs:isDefinedBy <http://data.nobelprize.org/terms/>;
  rdfs:label "Award File";
  rdfs:subClassOf foaf:Document .

nobel:Category a owl:Class;
  rdfs:comment "The Nobel Prize is given in six different categories.";
  rdfs:isDefinedBy <http://data.nobelprize.org/terms/>;
  rdfs:label "Nobel Prize category";
  rdfs:subClassOf skos:Concept;
  owl:oneOf (nobel:Chemistry nobel:Physics nobel:Literature nobel:Peace nobel:Economic_Sciences
      nobel:Physiology_or_Medicin) .

nobel:Chemistry a owl:Thing;
  rdfs:label "Chemistry" .

nobel:Economic_Sciences a owl:Thing;
  rdfs:label "Economic sciences" .

nobel:FileType a owl:Class;
  rdfs:comment "A file type indicates the nature of a prizeFile, for instance Acceptance Speach, Documentary, Press Release etc.";
  rdfs:isDefinedBy <http://data.nobelprize.org/terms/>;
  rdfs:label "File Type";
  rdfs:subClassOf skos:Concept .

nobel:Laureate a owl:Class;
  rdfs:comment "A laureate is a person or organization who recieves one or several Nobel Prizes.";
  rdfs:isDefinedBy <http://data.nobelprize.org/terms/>;
  rdfs:label "Laureate";
  rdfs:subClassOf foaf:Agent .

nobel:LaureateAward a owl:Class;
  rdfs:comment "The Nobel Prize is often divided to several laureates. LaureateAward captures the details of the award given to each laureate, such as share of the Nobel Prize, motivation etc.";
  rdfs:isDefinedBy <http://data.nobelprize.org/terms/>;
  rdfs:label "Laureate Award";
  rdfs:subClassOf dbpedia:Award .

nobel:Literature a owl:Thing;
  rdfs:label "Literature" .

nobel:NobelPrize a owl:Class;
  rdfs:comment "The Nobel Prize is a set of annual international awards bestowed in a number of categories by Scandinavian committees in recognition of cultural and scientific advances. The will of the Swedish chemist Alfred Nobel, the inventor of dynamite, established the prizes in 1895. The prizes in Physics, Chemistry, Physiology or Medicine, Literature, and Peace were first awarded in 1901. The Peace Prize is awarded in Oslo, Norway, while the other prizes are awarded in Stockholm, Sweden.";
  rdfs:isDefinedBy <http://data.nobelprize.org/terms/>;
  rdfs:label "Nobel Prize";
  rdfs:seeAlso <http://dbpedia.org/resource/Nobel_Prize>;
  rdfs:subClassOf dbpedia:Award .

nobel:Peace a owl:Thing;
  rdfs:label "Peace" .

nobel:Physics a owl:Thing;
  rdfs:label "Physics" .

nobel:Physiology_or_Medicin a owl:Thing;
  rdfs:label "Physiology or Medicin" .

nobel:PrizeFile a owl:Class;
  rdfs:comment "Some form of media related to the Nobel Prize.";
  rdfs:isDefinedBy <http://data.nobelprize.org/terms/>;
  rdfs:label "Prize File";
  rdfs:subClassOf foaf:Document .

nobel:awardFile a owl:ObjectProperty;
  rdfs:comment "Points to an AwardFile, that is some form of media related to the award for this laureate.";
  rdfs:domain nobel:LaureateAward;
  rdfs:isDefinedBy <http://data.nobelprize.org/terms/>;
  rdfs:label "awardFile";
  rdfs:range nobel:AwardFile .

nobel:category a owl:ObjectProperty;
  rdfs:comment "The category this Nobel Prize belongs to.";
  rdfs:domain nobel:NobelPrize;
  rdfs:isDefinedBy <http://data.nobelprize.org/terms/>;
  rdfs:label "category";
  rdfs:range nobel:Category .

nobel:contribution a owl:DatatypeProperty;
  rdfs:comment "The contribution for which the laureate was given the Nobel Prize.";
  rdfs:domain nobel:LaureateAward;
  rdfs:isDefinedBy <http://data.nobelprize.org/terms/>;
  rdfs:label "contribution";
  rdfs:range rdf:PlainLiteral .

nobel:field a owl:DatatypeProperty;
  rdfs:comment "The field within the category the Nobel Prize was awarded for.";
  rdfs:domain dbpedia:LaureateAward;
  rdfs:isDefinedBy <http://data.nobelprize.org/terms/>;
  rdfs:label "field";
  rdfs:range rdf:PlainLiteral .

nobel:fileType a owl:ObjectProperty;
  rdfs:comment "Points to an FileType, that is, what kind of prizeFile this is, for instance Acceptance Speach, Documentary, Press Release etc.";
  rdfs:domain nobel:PrizeFile;
  rdfs:isDefinedBy <http://data.nobelprize.org/terms/>;
  rdfs:label "fileType";
  rdfs:range nobel:FileType .

nobel:laureate a owl:ObjectProperty;
  rdfs:comment "Which laureates that recieve an award.";
  rdfs:domain nobel:LaureateAward;
  rdfs:isDefinedBy <http://data.nobelprize.org/terms/>;
  rdfs:label "laureate";
  rdfs:range nobel:Laureate .

nobel:laureateAward a owl:ObjectProperty;
  rdfs:comment "Connects each laureate with the part of the Nobel Prize, that is the LaureateAward, he or she recieved.";
  rdfs:domain nobel:Laureate;
  rdfs:isDefinedBy <http://data.nobelprize.org/terms/>;
  rdfs:label "laureateAward";
  rdfs:range nobel:LaureateAward;
  rdfs:subPropertyOf dbpedia:Award .

nobel:motivation a owl:DatatypeProperty;
  rdfs:comment "The motivation for why the laureate was given the Nobel Prize.";
  rdfs:domain nobel:LaureateAward;
  rdfs:isDefinedBy <http://data.nobelprize.org/terms/>;
  rdfs:label "motivation";
  rdfs:range rdf:PlainLiteral .

nobel:nobelPrize a owl:ObjectProperty;
  rdfs:comment "Points to the Nobel Prize recieved by a Laureate.";
  rdfs:domain nobel:Laureate;
  rdfs:isDefinedBy <http://data.nobelprize.org/terms/>;
  rdfs:label "nobelPrize";
  rdfs:range nobel:NobelPrize;
  rdfs:subPropertyOf dbpedia:Award .

nobel:prizeFile a owl:ObjectProperty;
  rdfs:comment "Points to an PrizeFile, that is some form of media related to the Nobel Prize.";
  rdfs:domain nobel:NobelPrize;
  rdfs:isDefinedBy <http://data.nobelprize.org/terms/>;
  rdfs:label "prizeFile";
  rdfs:range nobel:PrizeFile .

nobel:share a owl:DatatypeProperty;
  rdfs:comment "The share of a Nobel Prize given to a Laureate, may be 1, 2 or 4 corresponding to the whole prize, half the prize and a quarter of the prize.";
  rdfs:domain dbpedia:LaureateAward;
  rdfs:isDefinedBy <http://data.nobelprize.org/terms/>;
  rdfs:label "share";
  rdfs:range xsd:Integer .

nobel:university a owl:ObjectProperty;
  rdfs:comment "Points to the universities the Laureate was affiliated with during the period he did his contribution that laid the ground for the award.";
  rdfs:domain nobel:LaureateAward;
  rdfs:isDefinedBy <http://data.nobelprize.org/terms/>;
  rdfs:label "university";
  rdfs:range dbpedia:University .

nobel:year a owl:DatatypeProperty;
  rdfs:comment "The year a given Nobel Prize was given.";
  rdfs:domain dbpedia:Award;
  rdfs:isDefinedBy <http://data.nobelprize.org/terms/>;
  rdfs:label "year";
  rdfs:range xsd:Integer .

<http://www.nobelprize.org/> rdfs:label "Nobelprize.org" .
